\solution
Solving for BC
Given, 
\begin{align}
\vec{A} = \myvec{-3\\-5},
\vec{B} = \myvec{3\\-5},
\vec{C} = \myvec{-4\\-3} \\  
 \norm{\vec{B}-\vec{C}}\ &=  \sqrt{\brak{\vec{B}-\vec{C}}^{\top}\brak{\vec{B}-\vec{C}}} \\
 \vec{B}-\vec{C} &= \myvec{3 \\ -5} - \myvec{-4 \\ -3} \\
 \vec{B}-\vec{C} &= \myvec{7 \\ -2} \\
 \brak{\vec{B}-\vec{C}}^{\top} &= {\myvec{7 \\ -2}}^{\top} = \myvec{7 \ -2} \\
\brak{\vec{B}-\vec{C}}^{\top}\brak{\vec{B}-\vec{C}} &= \myvec{7 \ -2} \myvec{7 \\ -2}\\
             &= 49+4 \\
             &= 53 \\  
 \sqrt{\brak{\vec{B}-\vec{C}}^{\top}\brak{\vec{B}-\vec{C}}} &= \sqrt{53}	\\
	\implies \norm{\vec{B}-\vec{C}}\ &= \sqrt{53} 
\end{align}

Solving for AB 
Given, 
\begin{align}  
 \norm{\vec{A}-\vec{B}}\ &=  \sqrt{\brak{\vec{A}-\vec{B}}^{\top}\brak{\vec{A}-\vec{B}}} \\
 \vec{A}-\vec{B} &= \myvec{-3 \\ -5} - \myvec{3 \\ -5} \\
 \vec{A}-\vec{B} &= \myvec{-6 \\ 0} \\
 \brak{\vec{A}-\vec{B}}^{\top} &= {\myvec{-6 \\ 0}}^{\top} = \myvec{-6 \ -0} \\
\brak{\vec{A}-\vec{B}}^{\top}\brak{\vec{A}-\vec{B}} &= \myvec{-6 \ 0} \myvec{-6 \\ 0}\\
             &= 36 + 0 \\
             &= 36 \\  
	\sqrt{\brak{\vec{A}-\vec{B}}^{\top}\brak{\vec{A}-\vec{B}}} &= \sqrt{36}	\\
	\implies \norm{\vec{A}-\vec{B}}\ &= \sqrt{36} 
\end{align}

Solving for CA
Given, 
\begin{align}  
	\norm{\vec{C}-\vec{A}}\ &=  \sqrt{\brak{\vec{C}-\vec{A}}^{\top}\brak{\vec{C}-\vec{A}}} \\
 \vec{C}-\vec{A} &= \myvec{-4 \\ -3} - \myvec{-3 \\ -5} \\
 \vec{C}-\vec{A} &= \myvec{-1 \\ 2} \\
 \brak{\vec{C}-\vec{A}}^{\top} &= {\myvec{-1 \\ 2}}^{\top} = \myvec{-1 \ 2} \\
	\brak{\vec{C}-\vec{A}}^{\top}\brak{\vec{C}-\vec{A}} &= \myvec{-1 \ 2} \myvec{-1 \\ 2}\\
             &= 1 + 4 \\
             &= 5 \\  
	\sqrt{\brak{\vec{C}-\vec{A}}^{\top}\brak{\vec{C}-\vec{A}}} &= \sqrt{5}	\\
	\implies \norm{\vec{C}-\vec{A}}\ &= \sqrt{5} 
\end{align}

