\solution 
\\
From the given values of $\vec{A},\vec{B},\vec{C}$,\\
\begin{enumerate}

\item Finding the value of angle A
\begin{align}
	\vec{B}-\vec{A} &=\myvec{6\\0}
\end{align}
and 
\begin{align}
	\vec{C}-\vec{A}&= \myvec{-1\\+2}
\end{align}
also calculating the values of norms
\begin{align}
	\norm{\vec{B}-\vec{A}} &= \sqrt{36} &= 6\\
	\norm{\vec{C}-\vec{A}} &= \sqrt{5}
\end{align}
and by doing matrix multiplication we get,
\begin{align}
\begin{split}
	(\vec{B}-\vec{A})^{\top}(\vec{C}-\vec{A})&=\myvec{6&0}\myvec{-1\\+2}\\
	&=-6
\end{split}
\end{align}
so 
\begin{align}
	\cos{A}&= \frac{-6}{6 \sqrt{5}}\\
	&= \frac{-1}{\sqrt{5}}\\
	\implies A&=\cos^{-1}{\frac{-1}{\sqrt{5}}}
\end{align}




\item Finding the value of angle B
\begin{align}
	\vec{C}-\vec{B} &=\myvec{-7\\2}
\end{align}
and 
\begin{align}
	\vec{A}-\vec{B}&= \myvec{-6\\0}
\end{align}
also calculating the values of norms
\begin{align}
	\norm{\vec{C}-\vec{B}} &= \sqrt{5}\\
	\norm{\vec{A}-\vec{B}} &= \sqrt{53}
\end{align}
and by doing matrix multiplication we get,
\begin{align}
\begin{split}
	(\vec{C}-\vec{B})^{\top}(\vec{A}-\vec{B})&=\myvec{-7&2}\myvec{-6\\0}\\
	&= 42
\end{split}
\end{align}
so 
\begin{align}
	\cos{B}&= \frac{42}{\sqrt{36} \sqrt{53}}\\
	&= \frac{7}{\sqrt{53}}\\
	\implies B&=\cos^{-1}{\frac{7}{\sqrt{53}}}
\end{align}



\item Finding the value of angle C
\begin{align}
	\vec{A}-\vec{C} &=\myvec{1\\-2}
\end{align}
and 
\begin{align}
	\vec{B}-\vec{C}&= \myvec{7\\-2}
\end{align}
also calculating the values of norms
\begin{align}
	\norm{\vec{A}-\vec{C}} &= \sqrt{5}\\
	\norm{\vec{B}-\vec{C}} &= \sqrt{53}
\end{align}
and by doing matrix multiplication we get,
\begin{align}
\begin{split}
	(\vec{A}-\vec{C})^{\top}(\vec{B}-\vec{C})&=\myvec{1&-2}\myvec{7\\-2}\\
	&=11
\end{split}
\end{align}
so 
\begin{align}
	\cos{C}&= \frac{11}{\sqrt{5} \sqrt{53}}\\
	&= \frac{11}{\sqrt{265}}\\
	\implies C&=\cos^{-1}{\frac{11}{\sqrt{265}}}
\end{align}

\end{enumerate}
